SystemFD/Util.lean
@@ -4,3 +4,7 @@ def prefix_equal [BEq T] : List T -> List T -> Option (List T)
 | [], t => .some t
 | .cons _ _, [] => .none
 | .cons x1 t1, .cons x2 t2 => if x1 == x2 then prefix_equal t1 t2 else .none
+
+instance : Monad List where -- This seems fishy. Why doesn't lean have a Monad List instance?
+  pure a := List.cons a List.nil
+  bind l f := List.flatMap l f
